multiple changes... - updated map and set to new style. - arbitrary seq construction can now be accomplished through bless function.

src/ghost/map.fst
@@ -17,42 +17,58 @@
 
 module Tesseract.Ghost.Map
 
-   type map =
-      fun (key_t: Type) (val_t: Type) ->
-         key_t -> Tot (option val_t)
+   type map_g (key_t: Type) (value_t: Type) = 
+      key_t -> Tot (option value_t)
 
-   val empty: #key_t: Type -> #val_t: Type -> Tot (map key_t val_t)
-   let empty (key_t: Type) (val_t: Type) = 
-      fun _ -> 
-         None
+   val empty: 
+      #key_t: Type -> #value_t: Type -> 
+      Tot (map_g key_t value_t)
+   let empty (key_t: Type) (value_t: Type) = 
+      fun _ -> None
 
-   val mem: #key_t: Type -> #val_t: Type -> map key_t val_t -> key_t -> Tot bool
-   let mem m k = is_Some (m k)
+   val is_mem: 
+      #key_t: Type -> #value_t: Type -> 
+      map_g key_t value_t -> key_t -> Tot bool
+   let is_mem m k = 
+      is_Some (m k)
 
-   val lookup: #key_t: Type -> #val_t: Type -> m: map key_t val_t -> k: key_t{mem m k} -> Tot val_t
-   let lookup m k = 
-      match m k with
-         | Some v ->
-            v
+   val lookup: 
+      #key_t: Type -> #value_t: Type -> 
+      map: map_g key_t value_t -> k: key_t{is_mem map k} -> Tot value_t
+   let lookup map key = 
+      match map key with
+         | Some value ->
+            value
 
-   val domain: #key_t: Type -> #val_t: Type -> map key_t val_t -> Tot (Set.set key_t)
-   let domain m = 
-      Set.arbitrary (mem m)
+   val domain: 
+      #key_t: Type -> #value_t: Type -> 
+      map_g key_t value_t -> Tot (Set.set_g key_t)
+   let domain map = 
+      is_mem map
 
-   val update: #key_t: Type -> #val_t: Type -> map key_t val_t -> key_t -> val_t -> Tot (map key_t val_t)
-   let update (key_t: Type) (val_t: Type) m k v =
-      (fun kk ->
-         if k = kk then
-            Some v
+   val update: 
+      #key_t: Type -> #value_t: Type -> 
+      map_g key_t value_t -> key_t -> value_t 
+         -> Tot (map_g key_t value_t)
+   let update (key_t: Type) (value_t: Type) map key value =
+      (fun k ->
+         if key = k then
+            Some value
          else
-            m kk)
+            map k)
 
-   val add: #key_t: Type -> #val_t: Type -> m: map key_t val_t -> k: key_t{not (mem m k)} -> val_t -> Tot (map key_t val_t)
-   let add (key_t: Type) (val_t: Type) m k v =
-      update m k v
+   val add: 
+      #key_t: Type -> #value_t: Type -> 
+      map: map_g key_t value_t -> key: key_t{not (is_mem map key)} -> value_t 
+         -> Tot (map_g key_t value_t)
+   let add (key_t: Type) (value_t: Type) map key value =
+      update map key value
 
-   val subst: #key_t: Type -> #val_t: Type -> m: map key_t val_t -> k: key_t{mem m k} -> val_t -> Tot (map key_t val_t)
-   let subst (key_t: Type) (val_t: Type) m k v =
-      update m k v
+   val subst: 
+      #key_t: Type -> #value_t: Type -> 
+      map: map_g key_t value_t -> key: key_t{is_mem map key} -> value_t 
+         -> Tot (map_g key_t value_t)
+   let subst (key_t: Type) (value_t: Type) map key value =
+      update map key value
 
 // $vim-fst:32: vim:set sts=3 sw=3 et ft=fstar:,$
